code/Yazi.CRC32.Types.fst
@@ -1,0 +1,26 @@
+module Yazi.CRC32.Types
+
+module B = LowStar.Buffer
+module CB = LowStar.ConstBuffer
+module U32 = FStar.UInt32
+module U8 = FStar.UInt8
+module UInt = FStar.UInt
+
+open Lib.Seq
+
+type matrix_buf = B.lbuffer U32.t 32
+
+type table_buf = buf: CB.const_buffer U32.t{CB.length buf == 256}
+
+type crc32_data_dword (a b c d: U8.t) = res: U32.t{
+  let a' = UInt.to_vec (U8.v a) in
+  let b' = UInt.to_vec (U8.v b) in
+  let c' = UInt.to_vec (U8.v c) in
+  let d' = UInt.to_vec (U8.v d) in
+  let r' = UInt.to_vec (U32.v res) in
+  forall (i: nat{i < 32}). {:pattern r'.[i]}
+    (i >= 24 ==> r'.[i] == a'.[i - 24]) /\
+    (16 <= i /\ i < 24 ==> r'.[i] == b'.[i - 16]) /\
+    (8 <= i /\ i < 16 ==> r'.[i] == c'.[i - 8]) /\
+    (i < 8 ==> r'.[i] == d'.[i])
+}
